## [1]

$$
\begin{align*}
E[W] &= \int_0^{\infty} w \cdot \frac{1}{2^{k/2}\Gamma(k/2)}w^{k/2-1}e^{-w/2}dw\\
&= \int_0^{\infty} \frac{1}{2^{k/2}\Gamma(k/2)}w^{k/2}e^{-w/2}dw\\
&= \int_0^{\infty}\frac{1}{2^{k'/2-1}\Gamma(k'/2-1)}w^{k'/2-1}e^{-w/2}dw \quad &\left(\frac{k}{2} = \frac{k'}{2}-1とおいた\right)\\
&= \int_0^{\infty}\frac{1}{2^{k'/2}\cdot 2^{-1} \quad \frac{1}{k'/2-1}\Gamma(k'/2)}w^{k'/2-1}e^{-w/2}dw \quad &(\because \Gamma(\alpha+1) = \alpha \Gamma(\alpha))\\
&= (k'-2)\int_0^{\infty}\frac{1}{2^{k'/2}\Gamma(k'/2)}w^{k'/2-1}e^{-w/2}dw\\
&= k'-2 \\
&= k \\
\\
E[1/W] &= \int_0^{\infty} \frac{1}{w} \cdot \frac{1}{2^{k/2}\Gamma(k/2)}w^{k/2-1}e^{-w/2}dw\\
&= \int_0^{\infty} \frac{1}{2^{k/2}\Gamma(k/2)}w^{k/2-2}e^{-w/2}dw\\
&= \int_0^{\infty}\frac{1}{2^{k'/2+1}\Gamma(k'/2+1)}w^{k'/2-1}e^{-w/2}dw \quad &\left(\frac{k}{2}-2 = \frac{k'}{2}-1とおいた\right)\\
&= \int_0^{\infty}\frac{1}{2^{k'/2}\cdot 2 \quad (k'/2)\Gamma(k'/2)}w^{k'/2-1}e^{-w/2}dw \quad &(\because \Gamma(\alpha+1) = \alpha \Gamma(\alpha))\\
&= \frac{1}{k'}\int_0^{\infty}\frac{1}{2^{k'/2}\Gamma(k'/2)}w^{k'/2-1}e^{-w/2}dw\\
&= \frac{1}{k'}\\
&=\frac{1}{k-2}
\end{align*}
$$

なお $E[W]$, $E[1/W]$ が存在するためには、上記の途中式の自由度 $k/2+1$, 自由度 $k/2-1$ のカイ二乗分布が存在することになるので   
$$
\begin{align*}
k \gt 0\\
k/2+1 \gt 0\\
k/2-1 \gt 0\\
\\
\therefore k\gt 1
\end{align*}
$$
