## [1]

$$
\begin{align*}
E[Y] &= E[e^X]\\
&= \int e^x \cdot \frac{1}{\sqrt{2\pi\sigma^2}}\exp\left[-\frac{(x-\mu)^2}{2\sigma^2}\right]dx\\
&= \int \frac{1}{\sqrt{2\pi\sigma^2}}\exp\left[-\frac{(x-\mu)^2}{2\sigma^2} + x\right]dx\\
&= \int \frac{1}{\sqrt{2\pi\sigma^2}}\exp\left[-\frac{x^2 - 2(\mu + \sigma^2)x+ \mu^2}{2\sigma^2}\right]dx\\
&= \int \frac{1}{\sqrt{2\pi\sigma^2}}\exp\left[-\frac{\{x-(\mu + \sigma^2)\}^2 - (\mu + \sigma^2)^2+ \mu^2}{2\sigma^2}\right]dx\\
&= \int \frac{1}{\sqrt{2\pi\sigma^2}}\exp\left[-\frac{\{x-(\mu + \sigma^2)\}^2 -2\mu\sigma^2 - \sigma^4}{2\sigma^2}\right]dx\\
&= \int \frac{1}{\sqrt{2\pi\sigma^2}}\exp\left[-\frac{\{x-(\mu + \sigma^2)\}^2}{2\sigma^2} + \mu + \frac{\sigma^2}{2}\right]dx\\
&= \int \frac{1}{\sqrt{2\pi\sigma^2}}\exp\left[-\frac{\{x-(\mu + \sigma^2)\}^2}{2\sigma^2}\right]\exp\left[\mu + \frac{\sigma^2}{2}\right]dx\\
&= \exp\left[\mu + \frac{\sigma^2}{2}\right]\int \frac{1}{\sqrt{2\pi\sigma^2}}\exp\left[-\frac{\{x-(\mu + \sigma^2)\}^2}{2\sigma^2}\right]dx\\
&= \exp\left[\mu + \frac{\sigma^2}{2}\right]\cdot 1\\
&= \exp\left[\mu + \frac{\sigma^2}{2}\right]
\end{align*}
$$

## [2]

$$
\begin{align*}
E[Y^2] &= E[e^{2X}]\\
&= \int e^{2x} \cdot \frac{1}{\sqrt{2\pi\sigma^2}}\exp\left[-\frac{(x-\mu)^2}{2\sigma^2}\right]dx\\
&= \int \frac{1}{\sqrt{2\pi\sigma^2}}\exp\left[-\frac{(x-\mu)^2}{2\sigma^2} + 2x\right]dx\\
&= \int \frac{1}{\sqrt{2\pi\sigma^2}}\exp\left[-\frac{x^2 - 2(\mu + 2\sigma^2)x+ \mu^2}{2\sigma^2}\right]dx\\
&= \int \frac{1}{\sqrt{2\pi\sigma^2}}\exp\left[-\frac{\{x-(\mu + 2\sigma^2)\}^2 - (\mu + 2\sigma^2)^2+ \mu^2}{2\sigma^2}\right]dx\\
&= \int \frac{1}{\sqrt{2\pi\sigma^2}}\exp\left[-\frac{\{x-(\mu + 2\sigma^2)\}^2 -4\mu\sigma^2 - 4\sigma^4}{2\sigma^2}\right]dx\\
&= \int \frac{1}{\sqrt{2\pi\sigma^2}}\exp\left[-\frac{\{x-(\mu + \sigma^2)\}^2}{2\sigma^2} + 2\mu + 2\sigma^2\right]dx\\
&= \int \frac{1}{\sqrt{2\pi\sigma^2}}\exp\left[-\frac{\{x-(\mu + \sigma^2)\}^2}{2\sigma^2}\right]\exp\left[2\mu + 2\sigma^2\right]dx\\
&= \exp\left[2\mu + 2\sigma^2\right]\int \frac{1}{\sqrt{2\pi\sigma^2}}\exp\left[-\frac{\{x-(\mu + \sigma^2)\}^2}{2\sigma^2}\right]dx\\
&= \exp\left[2\mu + 2\sigma^2\right]\cdot 1\\
&= \exp\left[2\mu + 2\sigma^2\right]\\
\\
V[Y] &= E[Y^2]- E[Y]^2\\
&= \exp\left[2\mu + 2\sigma^2\right] - \exp\left[2\left(\mu + \frac{\sigma^2}{2}\right)\right]
\end{align*}
$$

## [3]
$Y=\exp(X)$とおくと、$X = \log{Y}$, $\frac{dX}{dY} = \frac{1}{Y}$である

$$
\begin{align*}
f(y) &= \frac{1}{\sqrt{2\pi \sigma^2}}\exp\left[-\frac{(\log{y} - \mu)^2}{2\sigma^2}\right]\cdot\frac{1}{y}\\
\end{align*}
$$
