## (1)

$X_{(j)}$の確率密度関数
$$
\begin{align*}
f_{X_{(j)}}(X_{(j)}=x) &= \frac{n!}{(j-1)!(n-j)!}F(x)^{j-1}f(x) (1-F(x))^{n-j}\\
&= \frac{n!}{(j-1)!(n-j)!}(1-e^{-\lambda x})^{j-1}\cdot \lambda e^{-\lambda x}\cdot (e^{-\lambda x})^{n-j}\\
&= \frac{n!}{(j-1)!(n-j)!}\lambda(1-e^{-\lambda x})^{j-1}e^{-\lambda x (n-j+1)}
\end{align*}
$$

j=1のとき
$$
f_{X_{(1)}}(X_{(1)}=x) = n\lambda e^{-\lambda n x}
$$
j = n のとき
$$
f_{X_{(n)}}(X_{(n)}=x) = n\lambda (1 - e^{-\lambda x})^{n-1}e^{-\lambda x}
$$

## (2)
$X_{(i)}$, $X_{(j)}$の同時確率密度関数
$$
\begin{align*}
f_{X_{(i)}, X_{(j)}}(X_{(i)}=x, X_{(j)}=y) &= \frac{n!}{(i-1)!(j-i-1)!(n-j)!}F(x)^{i-1}f(x)(F(y)-F(x))^{j-i-1}f(y) (1-F(y))^{n-j}
\end{align*}
$$  
i=1, j=nのとき
$$
\begin{align*}
f_{X_{(1)}, X_{(n)}}(X_{(1)}=x, X_{(n)}=y) &= n(n-1) \lambda e^{-\lambda x} (-e^{-\lambda y} + e^{-\lambda x})^{n-2}\lambda e^{-\lambda y}\\
&=n(n-1) \lambda^2 e^{-\lambda (x+y)} (-e^{-\lambda y} + e^{-\lambda x})^{n-2} 
\end{align*}
$$  

$X_{(1)}, \dots, X_{(n)}$の同時確率密度分布は、
$$\begin{align*}
f_{X_{(1)}, \dots, X_{(n)}}(X_{(1)} & =x_1, \dots, X_{(n)}=x_n) = n!f(x_1)\cdots f(x_n)\\
&= n!\lambda^n e^{-\lambda \sum_i^n x_i}
\end{align*}$$
