$$
\begin{align*}
\frac{1}{\sqrt{2\pi}}\int_{\infty}^{\infty}x^2e^{-x^2/2}dx &= \int_{\infty}^{\infty}x^2\cdot\frac{1}{\sqrt{2\pi}}e^{-x^2/2}dx\\
&= E[X^2]\quad(X\sim N(0, 1))
\end{align*}
$$
独立に標準正規分布に従う $X_1, X_2, \dots, X_n$ について、 大数の法則より
$$
\begin{align*}
\bar{G}_n &= \frac{1}{n}\sum_{i=1}^nX_i^2 \rightarrow E[X_i^2]\\
\\
\bar{G}_n & \rightarrow E[X_i^2] = 1
\end{align*}
$$

また、
$$
\begin{align*}
E[\bar{G_n}] &= \frac{1}{n}\sum_{i=1}^nE[X_i^2]\\
&= \frac{1}{n}\sum_{i=1}^nV[X_i]\\
&= 1\\
\\
V[\bar{G}_n] &= \frac{1}{n}\sum_{i=1}^nV[X_i^2]\\
&= \frac{1}{n}\sum_{i=1}^n (E[X^4] - E[X^2]^2)\\
&= \frac{1}{n}\sum_{i=1}^n (3 -1)\\
&= 2
\end{align*}
$$
より、
$\sqrt{n}(\bar{G}_n - 1) / \sqrt{2}$ は中心極限定理より$\sqrt{n}(\bar{G}_n - 1) / \sqrt{2} \rightarrow_p N(0, 1)$ に従う。  
したがって
$$
\sqrt{n}(\bar{G}_n - 1) \rightarrow_p N(0, 2)
$$