$$
\begin{align*}
E[F_n(x)] &= E\left[\frac{1}{n}\sum_{i=1}^nI(X_i\le x)\right]\\
&= \frac{1}{n}\sum_{i=1}^nE[I(X_i\le x)]\\
&= \frac{1}{n}\sum_{i=1}^nP(X\le x)\\
&= \frac{1}{n}\sum_{i=1}^nF(x)\\
&=F(x)\\
V[F_n(x)] &= V\left[\frac{1}{n}\sum_{i=1}^nI(X_i\le x)\right]\\
&= \frac{1}{n^2}\sum_{i=1}^nV[I(X_i\le x)]\\
&=\frac{1}{n^2}\sum_{i=1}^n\left( E[I(X_i\le x)^2] - E[X_i\le x]^2 \right)\\
&=\frac{1}{n^2}\sum_{i=1}^n\left( P(X\le x) - P(X\le x)^2 \right)\\
&=\frac{1}{n^2}\sum_{i=1}^nP(X\le x)(1 - P(X\le x))\\
&=\frac{1}{n^2}\sum_{i=1}^nF(x)(1 - F(x))\\
\\

E\left[\left(F_n(x) - E[F_n(x)]\right)^2\right] &= E\left[\left(F_n(x) - F(x)\right)^2\right]\\
&= V[F_n(x)]\\
&\rightarrow 0
\end{align*}
$$

中心極限定理より、 
$$
\frac{\sqrt{n}(F_n(x) - F(x))}{\sqrt{F(x)(1 - F(x))}}
$$
は、$N(0, 1)$ に従うので、
$$
\sqrt{n}(F_n(x) - F(x)) \sim N(0, F(x)(1 - F(x)))
$$