## [3]
$$\begin{align*}
1 - F(x) &= P(X \ge x)\\
&= \int_x^{\infty}f(t)dt
\end{align*}$$

$$\begin{align*}
\int_0^{\infty}1 - F(x) &= P(X \ge x)\\
&= \int_0^{\infty}\int_x^{\infty}f(t)dt dx
\end{align*}$$
??????????????????????????????

## [4]
$$\begin{align*}
f(x) &= \int_0^{\infty} g(x)h(\lambda)d\lambda\\
&= \int_0^{\infty} \lambda e^{-\lambda x} \cdot \frac{\beta^\alpha}{\Gamma(\alpha)}\lambda^\alpha e^{-\beta\lambda}d\lambda\\
&=\int_0^{\infty} \frac{\alpha\beta^\alpha}{\Gamma(\alpha + 1)}\lambda^{\alpha+1} e^{-(\beta+x)\lambda}d\lambda\\
&=\int_0^{\infty} \frac{\alpha\beta^\alpha}{\Gamma(\alpha + 1)}\cdot \frac{1}{(\beta + x)^{\alpha+1}}(\beta + x)^{\alpha+1} \cdot\lambda^{\alpha+1} e^{-(\beta+x)\lambda}d\lambda\\
&=\frac{\alpha\beta^\alpha}{(\beta + x)^{\alpha+1}}\int_0^{\infty} \frac{(\beta + x)^{\alpha+1}}{\Gamma(\alpha + 1)}\lambda^{\alpha+1} e^{-(\beta+x)\lambda}d\lambda\\
&= \frac{\alpha\beta^\alpha}{(\beta + x)^{\alpha+1}}\quad(x\ge0)
\end{align*}$$

## [5]
$$\begin{align*}
E[X] &= \int_0^{\infty}x\frac{\alpha\beta^\alpha}{(\beta + x)^{\alpha+1}}dx\\
&= \alpha\beta^\alpha\left(\left[-\frac{1}{\alpha}x\frac{1}{(\beta + x)^\alpha}\right]_0^{\infty} + \frac{1}{\alpha}\int_0^{\infty}\frac{1}{(\beta + x)^\alpha}dx\right)\\
&= \alpha\beta^\alpha\left(\left[-\frac{1}{\alpha}\frac{x}{(\beta + x)^\alpha}\right]_0^{\infty} + \frac{1}{\alpha}\left[-\frac{1}{\alpha-1}\frac{1}{(\beta + x)^{\alpha-1}}\right]_0^{\infty}\right)\\
&= -\beta^{\alpha}\left[\frac{x}{(\beta + x)^\alpha}+\frac{1}{\alpha-1}\frac{1}{(\beta + x)^{\alpha-1}}\right]_0^{\infty}
\end{align*}$$
$x\rightarrow\infty$のとき、第一項が収束するための条件 $\alpha\gt 1$  
$x\rightarrow\infty$のとき、第二項が収束するための条件 $\alpha - 1 \ge 0$  
よって、E[X]が収束するのは、$\alpha\gt 1$のとき  
このとき
$$
E[X] = -\beta^\alpha \cdot - \frac{1}{(\alpha-1)\beta^{\alpha - 1}} = \frac{\beta}{(\alpha-1)}
$$