## [1]
$$
\begin{align*}
E[U] &= E[X_1 + X_2]\\
&= E[X_1] + E[X_2] \quad (\because X_1 \perp X_2)\\
\\
E[X] &= \int_0^{\infty}\lambda x e^{-\lambda x}dx\\
&= \lambda\left[-\frac{x}{\lambda}e^{-\lambda x} - \frac{1}{\lambda^2}e^{-\lambda x}\right]_0^{\infty}\\
&= \frac{1}{\lambda}\\
\\
\therefore E[U] &= E[X_1 + X_2] = \frac{2}{\lambda}
\end{align*}
$$

## [2]
$U = X_1 + X_2$, $V = X_2$ とおくと、
$x_1 = u-v\ge 0$, $x_2 = v \ge 0 \Leftrightarrow 0\le v \le u$  
また、ヤコビアンは $\begin{vmatrix}\frac{\partial X_1}{\partial U} & \frac{\partial X_1}{\partial V}\\\frac{\partial X_2}{\partial U} & \frac{\partial X_2}{\partial V}\end{vmatrix} = 1$ より、

$$
\begin{align*}
f_{X_1X_2}(x_1, x_2) &= \lambda^2 e^{-\lambda(x_1+x_2)}\\
f_{UV}(u, v) &= \lambda^2e^{-\lambda u}
\end{align*}
$$

$V$ で積分して
$$
\begin{align*}
f_U(u) &= \int_0^uf_{UV}(u, v)dv\\
&= \int_0^u\lambda^2e^{-\lambda u}dv\\
&= \left[\lambda^2e^{-\lambda u}\cdot v\right]_0^u\\
&= \lambda^2ue^{-\lambda u}
\end{align*}
$$

## [3]
$$
\begin{align*}
E\left[\frac{1}{U}\right] &= \int_0^{\infty}\frac{1}{u}\lambda^2ue^{-\lambda u}du\\
&= \lambda\int_0^{\infty}\lambda e^{-\lambda u}du\\
&= \lambda
\end{align*}
$$

## [4]
$$
\begin{align*}
E\left[L(\alpha\bar{X}, \theta)\right] &= \int_0^{\infty}\left(\frac{\alpha u}{2\theta} + \frac{2\theta}{\alpha u} -2\right)\cdot \lambda^2ue^{-\lambda u}du\\
&=\frac{\alpha}{2\theta}\int_0^{\infty}\lambda^2u^2e^{-\lambda u}du + \frac{2\theta}{\alpha}\int_0^{\infty}\lambda^2e^{-\lambda u}du -2\int_0^{\infty}\lambda^2ue^{-\lambda u}du\\
&= \frac{\alpha}{2\theta}\cdot\frac{2}{\lambda} + \frac{2\theta}{\alpha}\cdot\lambda -2\\
&= \alpha + \frac{2}{\alpha} -2 \quad \left(\because \lambda =\frac{1}{\theta}\right)\\
\end{align*}
$$

$\alpha$ で微分して、$0$ とおくと

$$
\begin{align*}
&1 - \frac{2}{\alpha^2} = 0\\
&\alpha = \sqrt{2} \quad(\because \alpha \gt 0)
\end{align*}
$$